fix some se fallout

lean/src/bpf/se/symbolic_value.lean
@@ -15,7 +15,7 @@ variables {β γ : Type u} [smt.factory β γ] [smt.add_factory β γ] [smt.cons
   [smt.eq_factory β γ] [smt.not_factory β γ] [smt.and_factory β γ] [smt.redor_factory β γ] [smt.ult_factory β γ]
   [smt.ule_factory β γ] [smt.slt_factory β γ] [smt.sle_factory β γ]
 open smt.add_factory smt.const_factory smt.eq_factory smt.not_factory smt.and_factory smt.redor_factory smt.ult_factory
-     smt.slt_factory smt.sle_factory smt.ule_factory
+     smt.slt_factory smt.sle_factory smt.ule_factory factory.monad
 
 /-- Symbolic values of BPF registers -/
 inductive symvalue (β : Type u)
@@ -44,6 +44,9 @@ instance : factory bpf.value (symvalue β) γ :=
 def mk_scalar (imm : lsbvector 64) : state γ (symvalue β) :=
 symvalue.scalar <$> mk_const imm
 
+theorem le_mk_scalar {imm : lsbvector 64} : increasing (mk_scalar imm : state γ (symvalue β)) :=
+sorry
+
 theorem sat_mk_scalar ⦃g g' : γ⦄ ⦃e₁ : symvalue β⦄ ⦃imm : lsbvector 64⦄ :
   (mk_scalar imm).run g = (e₁, g') →
   sat g e₁ (bpf.value.scalar imm.nth) :=
@@ -56,6 +59,21 @@ theorem sat_mk_unknown ⦃g g' : γ⦄ ⦃e₁ : symvalue β⦄ ⦃v : erased bp
   (mk_unknown v).run g = (e₁, g') →
   sat g e₁ v.out :=
 sorry
+
+-- /-- Lift a constant function on 64 bits to expressions, losing precision.
+--     Computationally, this is just `mk_var`. -/
+-- def lift2_denote (f : i64 → i64 → i64) (e₁ e₂ : β) : state γ β :=
+-- mk_var $
+-- (factory.denote γ e₁).bind (λ (v₁ : Σ n, fin n → bool),
+--   (factory.denote γ e₂).bind (λ (v₂ : Σ n, fin n → bool),
+--     erased.mk $
+--       match v₁, v₂ with
+--       | ⟨64, b₁⟩, ⟨64, b₂⟩ := f b₁ b₂
+--       | _,        _        := default _
+--       end))
+
+-- def doALU : ∀ (op : bpf.ALU) (dst src : β), state γ β
+-- | op dst src       := lift2_denote (bpf.ALU.doALU_scalar op) dst src
 
 def doALU : Π (op : bpf.ALU) (a b : symvalue β), state γ (symvalue β)
 | bpf.ALU.ADD (symvalue.scalar x) (symvalue.scalar y) :=
@@ -79,7 +97,7 @@ theorem sat_doALU_check ⦃g g' : γ⦄ ⦃op : bpf.ALU⦄ ⦃e₁ e₂ : symval
   factory.sat g e₃ (⟨1, λ _, bpf.ALU.doALU_check op v₁ v₂ = tt⟩ : Σ (n : ℕ), fin n → bool) :=
 sorry
 
-def doJMP : Π (op : bpf.JMP) (a b : symvalue β), state γ β
+def doJMP : Π (op : JMP) (a b : symvalue β), state γ β
 | JMP.JEQ  (symvalue.scalar x) (symvalue.scalar y) := mk_eq x y
 | JMP.JNE  (symvalue.scalar x) (symvalue.scalar y) := mk_eq x y >>= mk_not
 | JMP.JSET (symvalue.scalar x) (symvalue.scalar y) := mk_and x y >>= mk_redor
@@ -93,9 +111,15 @@ def doJMP : Π (op : bpf.JMP) (a b : symvalue β), state γ β
 | JMP.JSGE (symvalue.scalar x) (symvalue.scalar y) := mk_sle y x
 | _ _ _ := mk_true
 
-def doJMP_check : Π (op : bpf.JMP) (a b : symvalue β), state γ β
+theorem doJMP_increasing {op : JMP} {a b : symvalue β} : increasing (doJMP op a b : state γ β) :=
+sorry
+
+def doJMP_check : Π (op : JMP) (a b : symvalue β), state γ β
 | _ (symvalue.scalar x) (symvalue.scalar y) := mk_true
 | _ _ _ := mk_false
+
+theorem doJMP_check_increasing {op : JMP} {a b : symvalue β} : increasing (doJMP_check op a b : state γ β) :=
+sorry
 
 end symvalue
 end se
